Foundation/Propositional/Kripke2/Logic/F.lean
@@ -1,0 +1,39 @@
+import Foundation.Propositional.Kripke2.Hilbert
+
+
+namespace LO.Propositional
+
+open Kripke2
+
+
+namespace Kripke2
+
+protected abbrev FrameClass.F : Kripke2.FrameClass := Set.univ
+
+abbrev trivialFrame : Kripke2.Frame where
+  World := Unit
+  Rel _ _ := True
+  root := ()
+  rooted := by simp
+
+end Kripke2
+
+
+namespace F
+
+open Hilbert.Corsi.Kripke2
+
+instance Kripke2.sound : Sound Propositional.F FrameClass.F := by
+  apply instFrameClassSound;
+  constructor;
+  tauto;
+
+instance : Entailment.Consistent Propositional.F := consistent_of_sound_frameclass FrameClass.F $ by
+  use Kripke2.trivialFrame;
+  apply Set.mem_setOf_eq.mpr;
+  simp;
+
+end F
+
+
+end LO.Propositional
